chore: remove Entails

src/Std/Sat/CNF/Basic.lean
@@ -46,20 +46,21 @@ def eval (a : α → Bool) (f : CNF α) : Bool := f.all fun c => c.eval a
 @[simp] theorem eval_append (a : α → Bool) (f1 f2 : CNF α) :
     eval a (f1 ++ f2) = (eval a f1 && eval a f2) := List.all_append
 
-instance : Entails α (Clause α) where
-  eval assign clause := Clause.eval assign clause
+def sat (a : α → Bool) (f : CNF α) : Prop := eval a f = true
+def unsat (f : CNF α) : Prop := ∀ a, eval a f = false
 
-instance : Entails α (CNF α) where
-  eval assign cnf := eval assign cnf
+theorem sat_def (a : α → Bool) (f : CNF α) : sat a f ↔ (eval a f = true) := by rfl
+theorem unsat_def (f : CNF α) : unsat f ↔ (∀ a, eval a f = false) := by rfl
 
-@[simp] theorem not_unsatisfiable_nil : ¬Unsatisfiable α ([] : CNF α) :=
-  fun h => by simp [Unsatisfiable, (· ⊨ ·)] at h
 
-@[simp] theorem sat_nil {assign : α → Bool} : assign ⊨ ([] : CNF α) := by
-  simp [(· ⊨ ·)]
+@[simp] theorem not_unsatisfiable_nil : ¬unsat ([] : CNF α) :=
+  fun h => by simp [unsat_def] at h
 
-@[simp] theorem unsat_nil_cons {g : CNF α} : Unsatisfiable α ([] :: g) := by
-  simp [Unsatisfiable, (· ⊨ ·)]
+@[simp] theorem sat_nil {assign : α → Bool} : sat assign ([] : CNF α) := by
+  simp [sat_def]
+
+@[simp] theorem unsat_nil_cons {g : CNF α} : unsat ([] :: g) := by
+  simp [unsat_def]
 
 namespace Clause
 
