src/Std/Sat.lean
@@ -4,5 +4,4 @@ Released under Apache 2.0 license as described in the file LICENSE.
 Authors: Henrik Böving
 -/
 prelude
-import Std.Sat.Basic
 import Std.Sat.CNF
